rocq-brick-libstdcpp/test/existing_specs/memory_addressof_cpp_proof.v
@@ -1,0 +1,58 @@
+
+Require Import skylabs.brick.libstdcpp.memory.spec.addressof.
+Require Import skylabs.brick.libstdcpp.test.existing_specs.memory_addressof_cpp.
+
+Require Import skylabs.brick.libstdcpp.lib.tactics.
+Require Import skylabs.brick.libstdcpp.cassert.spec.
+
+Require Import skylabs.auto.cpp.prelude.test.
+Require Import skylabs.cpp.spec.concepts.
+Require Import skylabs.cpp.spec.concepts.experimental.
+
+Module OverloadedAddress.
+  Import concepts.
+  cpp.class "overloaded_address" prefix "" from memory_addressof_cpp.source
+    dataclass { destructible }.
+End OverloadedAddress.
+
+NES.Begin memory_addressof_clients.
+  Section with_cpp.
+    Context `{Sigma : cpp_logic, sigma : genv}.
+
+    cpp.spec "test_public_addressof_int()" as test_public_addressof_int_spec from memory_addressof_cpp.source with (\post emp).
+    cpp.spec "test_public_addressof_overloaded()" as test_public_addressof_overloaded_spec from memory_addressof_cpp.source with (\post emp).
+    cpp.spec "test_internal_addressof_int()" as test_internal_addressof_int_spec from memory_addressof_cpp.source with (\post emp).
+    cpp.spec "test_internal_addressof_overloaded()" as test_internal_addressof_overloaded_spec from memory_addressof_cpp.source with (\post emp).
+
+    Lemma test_public_addressof_int_ok :
+      denoteModule memory_addressof_cpp.source |--
+        (▷ memory.addressof_spec "int" -∗
+         ▷ std.cassert.assert_fail_spec -∗
+         test_public_addressof_int_spec).
+    Proof. verify_spec. go $usenamed=true. Qed.
+
+    Lemma test_internal_addressof_int_ok :
+      denoteModule memory_addressof_cpp.source |--
+        (▷ memory.__addressof_spec "int" -∗
+         ▷ std.cassert.assert_fail_spec -∗
+         test_internal_addressof_int_spec).
+    Proof. verify_spec. go $usenamed=true. Qed.
+
+    Lemma test_public_addressof_overloaded_ok :
+      denoteModule memory_addressof_cpp.source |--
+        (▷ memory.addressof_spec "overloaded_address" -∗
+         ▷ OverloadedAddress.dtor_spec -∗
+         ▷ std.cassert.assert_fail_spec -∗
+         test_public_addressof_overloaded_spec).
+    Proof. verify_spec. go $usenamed=true. Qed.
+
+    Lemma test_internal_addressof_overloaded_ok :
+      denoteModule memory_addressof_cpp.source |--
+        (▷ memory.__addressof_spec "overloaded_address" -∗
+         ▷ OverloadedAddress.dtor_spec -∗
+         ▷ std.cassert.assert_fail_spec -∗
+         test_internal_addressof_overloaded_spec).
+    Proof. verify_spec. go $usenamed=true. Qed.
+  End with_cpp.
+NES.End memory_addressof_clients.
+
